#+TITLE:     Bayesian Biostatistics Learning note
#+AUTHOR:   [[https://wangcc.me][Chaochen Wang]]
#+EMAIL:     chaochen@wangcc.me
#+OPTIONS: d:(not "LOGBOOK") date:t e:t email:t f:t inline:t num:t
#+OPTIONS: timestamp:t title:t toc:t todo:t |:t


* Chapter 2 Bayes theorem: computing the posterior distribution

$$
p(\theta = 1 | y = 1) = 
\frac{p(y = 1 | \theta = 1)\times p(\theta=1)}
{p(y = 1 | \theta = 1)\times p(\theta = 1) +
p(y = 1 | \theta  = 0)\times p(\theta = 0)}
$$

In the above exporession, $p(\theta = 1)(p(\theta = 0))$ 
represents the prevalence (1 - prevalence) of a disease.
